dataplane/Correctness/Produces.thy
@@ -28,17 +28,11 @@ lemma to_zmset_list_diff[simp]:
   done
 
 lemma outputs_at_target_updates[simp]:
-  "outputs_at_target su (os(nid := (os nid)\<lparr> inter := A \<rparr>)) = outputs_at_target su os"
-  "outputs_at_target su (os(nid := (os nid)\<lparr> produ := B \<rparr>)) = outputs_at_target su os"
-  "outputs_at_target su (os(nid := (os nid)\<lparr> ocaps := C \<rparr>)) = outputs_at_target su os"
-  "outputs_at_target su (os(nid := (os nid)\<lparr> input := D \<rparr>)) = outputs_at_target su os"
-  "outputs_at_target su (os(nid := (os nid)\<lparr> inter := E \<rparr>)) = outputs_at_target su os"
-  "outputs_at_target su (os(nid := (os nid)\<lparr> nfron := F \<rparr>)) = outputs_at_target su os"
+  "outputs_at_target su (os(nid := (os nid)\<lparr> inter := A, nfron := F, produ := B, ocaps := C, input := D, inter := E  \<rparr>)) = outputs_at_target su os"
   unfolding outputs_at_target_def
   apply (rule ext)
   apply (auto split: prod.splits if_splits)
   done
-
 
 
 lemma to_zmset_BULK_BENQ[simp]:
@@ -50,76 +44,84 @@ lemma find_Some_singleton:
   "{x \<in> set xs . P x} = {x} \<Longrightarrow>
    find P xs = Some x"
   apply (induct xs)
-  apply simp_all
+   apply simp_all
   apply (auto 0 0 simp add:)
    apply blast
   apply (smt (verit, best) Collect_cong)
   done
-
-find_consts  "('a \<times> 'b) set \<Rightarrow> bool" name: inj
-
-(* 
-lemma graph_to_nxt_Src_from_Trg:
-  "(\<forall> nid p. card (Src_from_Trg su nid p) \<le> 1) \<Longrightarrow>
-   (\<forall> nid p. card (Trg_from_Src su nid p) \<le> 1) \<Longrightarrow>
-   graph_to_nxt su ((nid' :: 'nid :: enum), (p' :: 'p :: enum)) = Some (nid :: 'nid, p :: 'p) \<longleftrightarrow> Src_from_Trg su nid p = {(nid', p' :: 'p)}"
-  unfolding graph_to_nxt_def Src_from_Trg_def
-  apply (auto simp add: card_eq_Suc_0_ex1 le_eq_less_or_eq)
-  subgoal for nid p
-    by (metis (mono_tags, lifting) find_SomeD(1) is_empty_antichain_simp old.prod.case old.prod.inject)
- *)
 
 lemma eq_singletonD:
   "{x. P x} = {x} \<Longrightarrow> P x"
   by auto
 
 lemma in_op_conn_graph_to_nxt_iff:
-  "single_valued (op_conn su) \<Longrightarrow>
-   graph_to_nxt su (nid, p) = Some (nid', p') \<longleftrightarrow> ((nid, p), nid', p') \<in> op_conn su"
-  unfolding graph_to_nxt_def op_conn_def
+  "bi_unique (op_conn su) \<Longrightarrow>
+   graph_to_nxt su (nid, p) = Some (nid', p') \<longleftrightarrow> op_conn su (nid, p) (nid', p')"
+  unfolding graph_to_nxt_def
   apply (auto simp add: is_empty_antichain_iff split: prod.splits)
   subgoal
-    apply (auto simp add: single_valued_def dest!: find_SomeD' split: prod.splits)
+    apply (auto simp add: dest!: find_SomeD' split: prod.splits)
     done
   subgoal
     apply (rule find_Some_singleton)
-    apply (auto simp add: single_valued_def split: prod.splits)
+    apply (auto simp add: bi_unique_def split: prod.splits)
     done
   done
 
 lemma graph_to_nxt_not_Ex_op_conn[simp]:
   "graph_to_nxt su (nid, p) = None \<longleftrightarrow>
-   \<not> (\<exists> nid' p'. ((nid, p), nid', p') \<in> op_conn su)"
-  unfolding graph_to_nxt_def op_conn_def
+   \<not> (\<exists> nid' p'. op_conn su (nid, p) (nid', p'))"
+  unfolding graph_to_nxt_def
   apply (auto simp add: is_empty_antichain_iff find_None_iff dest!: find_SomeD' split: prod.splits)
   done
 
-lemma
-    "outputs_at_target su (os((nid :: 'n :: enum) := (os nid)\<lparr> outpu := (\<lambda>(p :: 'p). oputs p) \<rparr>)) (nid', p') =
-     (let S = {p''. su (Loc nid (Src p'')) (Loc nid' (Trg p')) \<noteq> {}\<^sub>A} in if S \<noteq> {} then oputs (Set.the_elem S) else outputs_at_target su os (nid', p'))"
+lemma the_elem_bi_unique_op_conn:
+  "the_elem {(nid', p'). su (Loc nid' (Src p')) (Loc nid (Trg p)) \<noteq> {}\<^sub>A} = (nid', p') \<Longrightarrow>
+   su (Loc nid'' (Src p'')) (Loc nid (Trg p)) \<noteq> {}\<^sub>A \<Longrightarrow>
+   bi_unique (op_conn su) \<Longrightarrow>
+   nid' = nid'' \<and> p' = p''"
+  apply (subst (asm) the_elem_image_unique[where f=id, simplified, of _  "(nid'', p'')"])
+    apply blast
+  unfolding bi_unique_def
+   apply auto
+  done
+
+
+lemma outputs_at_target_outpu_if:
+  "bi_unique (op_conn su) \<Longrightarrow>
+   os' = os(nid := (os nid)\<lparr> outpu := X \<rparr>) \<Longrightarrow>
+   outputs_at_target su os' (nid', p') = 
+  (let S = {p. op_conn su (nid, p) (nid', p')} in if S \<noteq> {} then let p = the_elem S in X p else outputs_at_target su os (nid', p'))"
   unfolding outputs_at_target_def
-  apply (clarsimp split: prod.splits if_splits)
-  subgoal for a
-    unfolding  le_eq_less_or_eq
-    apply (auto simp add: card_eq_0_iff card_1_singleton_iff)
-    subgoal for p nid'
-      apply hypsubst_thin
-      apply (rule FalseE)
-      oops
-
-lemma
-  "single_valued ((op_conn su)\<inverse>) \<Longrightarrow>
-   summ sg (Loc nid'' (Src p'')) (Loc nid' (Trg p')) \<noteq> {}\<^sub>A \<Longrightarrow>
-   the_elem {(nid'', p''). ((nid'', p''), nid', p') \<in> op_conn (summ sg)} = (nid, p) \<Longrightarrow>
-   ((nid, p), nid', p') \<in> op_conn su"
-  unfolding graph_to_nxt_def op_conn_def the_elem_def
-  apply (auto simp add: single_valued_def dest!: split: prod.splits)
+  apply (auto split: prod.splits)
   subgoal
-    oops
-
+    apply (drule the_elem_bi_unique_op_conn)
+      apply assumption+
+    apply auto
+    done
+  subgoal for x2 a b x
+    apply (subst the_elem_image_unique[where f=id, simplified, of _ "b"])
+      apply fast
+    unfolding bi_unique_def
+     apply auto
+    apply (subst (asm) the_elem_image_unique[where f=id, simplified, of _  "(a, b)"])
+      apply blast
+     apply auto
+    done
+  subgoal for x2 a b x
+    apply (subst the_elem_image_unique[where f=id, simplified, of _ "x"])
+      apply fast
+    unfolding bi_unique_def
+     apply auto
+    apply (subst (asm) the_elem_image_unique[where f=id, simplified, of _  "(_, x)"])
+      apply blast
+     apply auto
+    done
+  done
 
 lemma dataplane_tracker_inv_produces_drops:
   fixes drops :: "'p :: {enum,linorder} \<Rightarrow> 't :: {ccompare,canonically_ordered_monoid_add,ordered_ab_semigroup_monoid_add_imp_le,bot} list"
+  assumes D: "dataflow_topology (summ sg) (-+-)"
   shows
     "noutput = (\<lambda> p . outpu (os nid) p @ oputs p) \<Longrightarrow>
    nocaps = (\<lambda> p . list_diff (ocaps (os nid) p) (drops p)) \<Longrightarrow>
@@ -146,7 +148,7 @@ lemma dataplane_tracker_inv_produces_drops:
       apply (rule exI[of _ 
             "(\<lambda> l. case l of 
        Loc nid' (Src p') \<Rightarrow> if nid' = nid then caps l - to_zmset (drops p') else caps l 
-     | Loc nid' (Trg p') \<Rightarrow>  caps l + zmset (map snd (filter (\<lambda> (p'', _, _). (graph_to_nxt (summ sg)) (nid, p'') = Some (nid', p')) produs)))"])
+     | Loc nid' (Trg p') \<Rightarrow> caps l + zmset (map snd (filter (\<lambda> (p'', _, _). (graph_to_nxt (summ sg)) (nid, p'') = Some (nid', p')) produs)))"])
       apply (intro conjI)
       subgoal premises prems
         using prems(6)
@@ -171,24 +173,24 @@ lemma dataplane_tracker_inv_produces_drops:
             apply (rule map_cong)
             subgoal
               apply (rule filter_cong)
-               apply (auto split: prod.splits simp add: op_conn_def )
+               apply (auto split: prod.splits simp add: )
               subgoal
-                apply (drule GS(8)[unfolded op_conn_def single_valued_def, simplified, rule_format])
+                apply (drule conjunct2[OF GS(7)[unfolded bi_unique_def, simplified, rule_format], rule_format])
                  apply assumption
                 apply auto
                 apply hypsubst_thin
                 apply (subst (asm) the_elem_image_unique[where f=id, simplified])
                   apply blast
                  apply clarsimp
-                using GS(8)[unfolded op_conn_def single_valued_def, simplified, rule_format] apply blast
-                apply auto
+                 apply (drule conjunct2[OF GS(7)[unfolded bi_unique_def, simplified, rule_format], rule_format])              
+                  apply auto
                 done
               subgoal
                 apply (subst (asm) the_elem_image_unique[where f=id, simplified])
                   apply blast
                  apply clarsimp
-                using GS(8)[unfolded op_conn_def single_valued_def, simplified, rule_format] apply blast
-                apply auto
+                 apply (drule conjunct2[OF GS(7)[unfolded bi_unique_def, simplified, rule_format], rule_format])
+                  apply auto
                 done
               done
             apply simp
@@ -197,11 +199,11 @@ lemma dataplane_tracker_inv_produces_drops:
             apply (subst filter_False)
              apply simp_all
             subgoal
-              apply (auto split: prod.splits simp add: op_conn_def )
+              apply (auto split: prod.splits simp add: )
               apply (subst (asm) the_elem_image_unique[where f=id, simplified])
                 apply blast
                apply clarsimp
-              using GS(8)[unfolded op_conn_def single_valued_def, simplified, rule_format] apply blast+
+              using conjunct2[OF GS(7)[unfolded bi_unique_def, simplified, rule_format], rule_format] apply blast+
               done
             done
           done
@@ -213,10 +215,299 @@ lemma dataplane_tracker_inv_produces_drops:
         subgoal for l
           apply (drule spec[of _ l])
           apply (drule sym)
-          apply (auto simp add:  c_pts_change_multiplicities split: location.splits port.splits; hypsubst_thin)
+          apply (auto simp add: extract_prog_def  c_pts_change_multiplicities split: location.splits port.splits; hypsubst_thin)
+          subgoal premises aux for nid' p'
+            apply (simp add: filter_map monoid_add_class.sum_list_distinct_conv_sum_set zmset_concat filter_concat map_concat comp_def)
+            apply (subst (1 2) comm_monoid_add_class.sum.subset_diff[where B="{nid}"])
+              apply simp_all
+            unfolding extract_progress_def obtain_progress_def
+            apply (simp add: List.map_filter_def split_beta filter_map monoid_add_class.sum_list_distinct_conv_sum_set zmset_concat filter_concat map_concat comp_def split: option.splits)
+            apply (rule arg_cong[where f=zmset])
+            apply (rule map_cong)
+             apply simp_all
+             apply (rule filter_cong)
+              apply (auto simp add: in_op_conn_graph_to_nxt_iff[OF GS(7)] split: prod.splits option.splits dest: conjunct1[OF GS(7)[unfolded bi_unique_def, simplified, rule_format], rule_format])
+            done
+          subgoal premises aux for nid'
+            apply (simp add: filter_map monoid_add_class.sum_list_distinct_conv_sum_set zmset_concat filter_concat map_concat comp_def)
+            apply (subst (1 2) comm_monoid_add_class.sum.subset_diff[where B="{nid}"])
+              apply simp_all
+            unfolding extract_progress_def obtain_progress_def
+            apply (simp add: to_zmset_filter List.map_filter_def split_beta filter_map monoid_add_class.sum_list_distinct_conv_sum_set zmset_concat filter_concat map_concat comp_def split: option.splits)
+            apply (subst comm_monoid_add_class.sum.subset_diff[where B="{nid'}"])
+              apply auto
+            done
           subgoal for nid' p'
+            apply (simp add: filter_map monoid_add_class.sum_list_distinct_conv_sum_set zmset_concat filter_concat map_concat comp_def)
+            apply (subst (1 2) comm_monoid_add_class.sum.subset_diff[where B="{nid}"])
+              apply simp_all
+            unfolding extract_progress_def obtain_progress_def
+            apply (simp add: to_zmset_filter List.map_filter_def split_beta filter_map monoid_add_class.sum_list_distinct_conv_sum_set zmset_concat filter_concat map_concat comp_def split: option.splits)
+            done
+          done
+        done
+      subgoal premises prems
+        using prems(9) apply -
+        unfolding front_inv_def
+        apply simp
+        done
+      subgoal premises prems
+        apply (subgoal_tac "(\<forall> p nid' p'. \<forall> t \<in> snd ` set (oputs p). summ sg (Loc nid (Src p)) (Loc nid' (Trg p')) \<noteq> {}\<^sub>A \<longrightarrow> frontier_less_equal (ifrontier (summ sg) (+) (pt_tr sg) (Loc nid' (Trg p'))) t)")
+        subgoal
+          using prems(11) apply -
+          unfolding chnls_imp_front_inv_def Let_def BULK_BENQ_def apply -
+          apply (auto simp add: outputs_at_target_def split: if_splits prod.splits)
+              apply (smt (verit) Collect_cong Un_iff mem_Collect_eq snd_conv split_cong)
+             apply (smt (verit) Collect_cong Un_iff mem_Collect_eq snd_conv split_cong)
+          subgoal
+            apply (drule spec)+
+            apply auto
+               apply force
+              defer
+              apply force+
+            done
+          subgoal
+            apply (drule sym)
+            apply (drule the_elem_bi_unique_op_conn)
+              apply assumption
+            using GS(7) apply assumption
+            apply auto
+            apply (drule spec2, drule spec, drule mp, assumption)
+            apply (drule bspec)
+             apply simp
+            apply simp
+            done
+          subgoal
+            apply (drule sym)
+            apply (drule the_elem_bi_unique_op_conn)
+              apply assumption
+            using GS(7) apply assumption
+            apply auto
+            apply (drule spec2, drule spec, drule mp, assumption)
+            apply (drule bspec)
+             apply simp
+            apply simp
+            done
+          done
+        subgoal
+          apply safe
+          subgoal for p nid' p' _ d t
+            apply simp
+            using temp(3,7,9) apply -
+            unfolding Src_caps_inv_def
+            apply (drule spec2[of _ nid p])
+            unfolding c_pts_inv_def
+            apply (drule spec[of _ "Loc nid (Src p)"])
+            apply simp
+            apply (rule frontier_less_equal_le_trans[rotated])
+             apply (rule frontier_less_equal_change_multiplicities[OF D, where A="extract_prog enum_class.enum (graph_to_nxt (summ sg)) os"])
+            subgoal 
+              apply safe
+              subgoal for l t m
+                apply (subst (asm) (2) extract_prog_def)
+                apply clarsimp
+                subgoal for nid''
+                  using temp(15)[unfolded extract_prog_changes_above_impl_inv_def, rule_format, of Nil nid'', simplified, unfolded changes_above_impl_inv_def]
+                  apply auto
+                  done
+                done
+              done
+            subgoal
+              apply (rule frontier_less_equal_ifrontierI[of _ 0 "Loc nid (Src p)", simplified, OF D])
+              subgoal
+                apply (rule path_weight_direct_0path[OF dataflow_topology.axioms(1)[OF D]])
+                apply (meson GS(2,7) in_op_conn_graph_to_nxt_iff op_conn.simps)
+                done
+              apply simp
+              apply (meson frontier_less_equal_zcount_pos snd_image_mp zcount_to_zmset_gt_0)
+              done
+            done
+          done
+        done
+      subgoal premises prems
+        using prems(12,2) apply -
+        unfolding change_deltas_inv_def
+        apply auto
+        done
+      subgoal premises prems
+        unfolding extract_prog_changes_above_impl_inv_def
+        apply (auto 0 0)
+        subgoal for xs
+          using prems(14)[unfolded extract_prog_changes_above_impl_inv_def, rule_format, of xs] D temp(1,7,9,2) GS(2,7) apply -
+          apply (induct xs arbitrary: os sg rule: rev_induct)
+          subgoal for os sg
+            apply simp
+            unfolding changes_above_impl_inv_def
+            apply safe
+            subgoal for l t m
+              apply (clarsimp simp add: split_beta)
+              apply (subst (asm) (2) obtain_progress_def)
+              apply (subst (asm) (2) extract_progress_def)
+              apply (clarsimp simp add: Misc.set_map_filter image_iff split_beta split: option.splits; hypsubst_thin?)
+              subgoal for p' m
+                apply (drule meta_spec)+
+                apply (drule bspec)
+                 back
+                unfolding extract_progress_def obtain_progress_def
+                 apply (clarsimp del: disjCI simp add: Misc.set_map_filter image_iff split_beta split: option.splits; hypsubst_thin?)
+                 apply fast
+                apply simp
+                done
+              subgoal for p' 
+                apply (drule meta_spec)+
+                apply (drule bspec)
+                 back
+                unfolding extract_progress_def obtain_progress_def
+                 apply (clarsimp simp add: Misc.set_map_filter image_iff split_beta split: option.splits; hypsubst_thin?)
+                 apply blast
+                apply simp
+                done
+              subgoal for p' 
+                apply (rule frontier_less_equal_le_trans[rotated])
+                 apply (rule frontier_less_equal_change_multiplicities[where A="extract_prog enum_class.enum (graph_to_nxt (summ sg)) os"])
+                  apply assumption
+                subgoal 
+                  apply safe
+                  apply (subst (asm) (2) extract_prog_def)
+                  apply clarsimp
+                  subgoal
+                    by force
+                  done
+                subgoal
+                  apply (rule frontier_less_equal_ifrontierI[of _ 0 "Loc nid (Src p')", simplified])
+                    apply assumption
+                  subgoal
+                    apply (rule graph.path_weight_refl)
+                    apply (rule dataflow_topology.axioms(1))
+                    apply auto
+                    done
+                  subgoal
+                    unfolding Src_caps_inv_def
+                    apply (drule spec2[of _ nid p'])
+                    unfolding c_pts_inv_def
+                    apply (drule spec[of _ "Loc nid (Src p')"])
+                    apply simp
+                    apply (subgoal_tac "t \<in> set (ocaps (os nid) p')") 
+                    subgoal
+                      by (simp add: frontier_less_equal_zcount_pos)
+                    subgoal
+                      by force
+                    done
+                  done
+                done
+              subgoal for p nid' p'
+                apply (drule meta_spec[of _ nid])
+                apply (drule spec2, drule spec2, drule mp, assumption)
+                apply (drule bspec[of _ _ "(Loc nid' (Trg p'), _, _)"])
+                 apply simp_all
+                unfolding extract_progress_def obtain_progress_def
+                apply (clarsimp del: disjCI simp add: Misc.set_map_filter image_iff split_beta split: option.splits; hypsubst_thin?)
+                apply (rule disjI2)+
+                apply (rule exI[of _ p])
+                apply (intro conjI impI allI)
+                 apply (rule exI[of _ nid'])
+                 apply (rule exI[of _ p'])
+                 apply simp
+                apply auto
+                done
+              subgoal for p t' b nid' p'
+                apply (subgoal_tac "graph_to_nxt (summ sg) (nid, p) = Some (nid', p')")
+                subgoal
+                  apply (drule spec2[of _ nid' p'])
+                  apply (drule mp)
+                   apply assumption
+                  apply clarsimp
+                  apply hypsubst_thin
+                  apply (drule bspec)
+                   apply assumption
+                  apply clarsimp
+                  unfolding Src_caps_inv_def
+                  apply (drule spec2[of _ nid p])
+                  unfolding c_pts_inv_def
+                  apply (drule spec[of _ "Loc nid (Src p)"])
+                  apply simp
+                  apply (rule frontier_less_equal_le_trans[rotated])
+                   apply (rule frontier_less_equal_change_multiplicities[where A="extract_prog enum_class.enum (graph_to_nxt (summ sg)) os"])
+                    apply assumption
+                  subgoal
+                    apply safe
+                    apply (subst (asm) (2) extract_prog_def)
+                    apply clarsimp
+                    apply fastforce
+                    done
+                  apply (rule frontier_less_equal_ifrontierI[of _ 0 "Loc nid (Src p)", simplified])
+                    apply assumption
+                  subgoal
+                    apply (rule path_weight_direct_0path[OF dataflow_topology.axioms(1)[]])
+                     apply assumption
+                    apply auto
+                    done
+                  apply simp
+                  apply (meson frontier_less_equal_zcount_pos zcount_to_zmset_gt_0)
+                  done
+                subgoal premises temp2
+                  using temp2(10) apply -
+                  unfolding graph_to_nxt_def
+                  apply simp
+                  apply (rule find_Some_singleton)
+                  apply (auto simp add: is_empty_antichain_iff)
+                  using temp2(8)
+                   apply (metis Pair_inject bi_uniqueDr op_conn.simps)+
+                  done
+                done
+              done
+            done
+          subgoal premises prems for nid' xs os sg
+            using prems(2-) apply -
+            using prems(1) apply -
+            apply (drule meta_spec[of _ "sg\<lparr> pt_tr :=  change_multiplicities (summ sg) (extract_prog [nid'] (graph_to_nxt (summ sg)) os) (pt_tr sg) \<rparr>"])
+            apply (drule meta_spec[of _ "os( nid' := fst (obtain_progress (os nid')) )"])
+            apply (drule meta_mp)
+            subgoal 
+              using prems(2) by auto
+            apply (drule meta_mp)
+            subgoal 
+              using prems(3) by auto
+            apply (drule meta_mp)
+            subgoal for nid''
+              apply (auto simp add:  )
+              apply (drule meta_spec[of _ nid''])
+              apply (drule meta_mp)
+               apply simp
+              apply (metis (no_types, opaque_lifting) change_multiplicities_append_alt change_multiplicities_comm)
+              done
+            apply auto
+            apply (drule meta_mp)
+            subgoal 
+              using prems(7) apply -
+              unfolding Src_caps_inv_def obtain_progress_def
+              apply auto
+              done
+            apply (metis (no_types, lifting) change_multiplicities_append_alt change_multiplicities_comm)
+            done
+          done
+
           
 
+            find_theorems produs
+
+end
+  apply (rule frontier_less_equal_ifrontier_from_Src[where s=0 and nid=nid and nt="graph_to_nxt (summ sg)" and p=p and os=os, simplified, OF D])
+  defer
+
+  using prems(14) apply assumption
+
+
+
+  find_theorems extract_prog_changes_above_impl_inv
+
+  thm conjunct2[OF GS(7)[unfolded bi_unique_def, simplified, rule_format], rule_format]
+
+  using GS(7)
+
+  thm in_op_conn_graph_to_nxt_iff[OF GS(7)]
+
+  find_theorems graph_to_nxt Some
 
 
 
