dataplane/Examples/Batch_op_Correctness.thy
@@ -70,9 +70,9 @@ abbreviation "G f ip_state os2 \<equiv> Comp [(0 :: 2, 1) \<mapsto> (0, 1)] (l1 
 
 abbreviation "test_op \<equiv> compile_dataflow (\<lambda> _. []) (G (\<lambda> b. if b = [] then trace (STR ''Empty batch! ! !'') [] else [Max (set b)]) (init_input_state default_internal_summary (\<lambda> _. inps_test)) (init_operator_state_ty2 default_internal_summary) )"
 
-(* value [GHC] "lmap (\<lambda> io. case io of VOut p (x, t) \<Rightarrow> (projr x, t)) (trace_exec test_op)"
+value [GHC] "lmap (\<lambda> io. case io of VOut p (x, t) \<Rightarrow> (projr x, t)) (trace_exec test_op)"
 value [GHC] "check_prefix 100 [((1, 1), (Inr 10, MyPair 1 1)), ((1, 1), (Inr 7, MyPair 0 1)),((1, 1), (Inr 3, MyPair 1 0))] test_op"
-value [GHC] "check_prefix 100 [((1, 1), (Inr 7, MyPair 0 1)), ((1, 1), (Inr 10, MyPair 1 1)), ((1, 1), (Inr 3, MyPair 1 0))] test_op" *)
+value [GHC] "check_prefix 100 [((1, 1), (Inr 7, MyPair 0 1)), ((1, 1), (Inr 10, MyPair 1 1)), ((1, 1), (Inr 3, MyPair 1 0))] test_op"
 (* value [GHC] "check_prefix 100 [((1, 1), (Inr 3, MyPair 1 0)), ((1, 1), (Inr 10, MyPair 1 1)), ((1, 1), (Inr 7, MyPair 0 1))] test_op"
  *)
 section \<open>Generalized Correctness\<close>
@@ -123,7 +123,7 @@ lemma weights_to_graph_fun_to_next[simp]:
 lemma dataflow_tree_to_graph_to_my_summ[simp]:
   "dataflow_tree_to_graph (Comp [(0, 1) \<mapsto> (0, 1)] (Logic op1 default_internal_summary) (Logic op2 default_internal_summary)) = (my_summ :: (2, 1) location \<Rightarrow> (2, 1) location \<Rightarrow> _ list)"
   unfolding dataflow_tree_to_graph_def Let_def default_internal_summary_def comp_def                                               
-(*   apply (simp only: split: if_splits prod.splits)
+  apply (simp only: split: if_splits prod.splits)
   apply (intro allI impI conjI)
   subgoal
     apply clarsimp
@@ -156,10 +156,13 @@ lemma dataflow_tree_to_graph_to_my_summ[simp]:
           by (cases lp1; cases lp2; simp add: incomparable_def if_distrib split: if_splits)
         done
       subgoal for nid
-      by (clarsimp simp add: image_iff split_beta split: prod.splits if_splits port.splits)
+        by (clarsimp simp add: image_iff split_beta split: prod.splits if_splits port.splits)
+      subgoal 
+        unfolding bi_unique_def
+        apply (clarsimp simp add: image_iff split_beta split: prod.splits if_splits port.splits)
     done
-  done *)
-  sorry
+  done 
+  done
 
 definition "coll inps t = list_of (lmap (\<lambda> e. case e of Data t d \<Rightarrow> d) (lfilter (\<lambda> e. case e of Data t' d \<Rightarrow> t = t' | _ \<Rightarrow> False) inps))"
 
@@ -259,7 +262,7 @@ lemma in_cimage_cset_from_list[simp]:
 
 lemma outputs_at_target_my_summ:
   "outputs_at_target (antichain_from_list oo my_summ) os = (\<lambda> p. if p = (1, 0) then outpu (os 0) 0 else [])"
-  unfolding outputs_at_target_def my_summ_def op_conn_def
+  unfolding outputs_at_target_def my_summ_def
   apply (rule ext)
   apply (auto simp add: antichain_from_list_singleton split: prod.splits if_splits)
   subgoal for nid
@@ -537,14 +540,15 @@ proof (coinduction arbitrary: os sg ip_state bt_state chns cbufs inps SP SO S D 
                       apply (clarsimp simp add: SIM1(1,2) comp_def)
                       apply (drule spec2[of _ 1 0], drule mp)
                        back
-                       apply (simp_all add: op_conn_def)
+                       apply (simp_all add: bi_unique_def)
                       subgoal premises
                         unfolding graph_to_nxt_def
                         apply auto
                         subgoal
                           unfolding my_summ_def inj_on_def
-                          apply clarsimp
-                          sorry
+                          apply (auto simp add: antichain_from_list_singleton is_empty_antichain_iff split: prod.splits if_splits intro!: find_Some_singleton)
+                          apply (metis dataflow_topology_from_tree.set_antichain_0 empty_antichain.rep_eq insert_not_empty)
+                          done
                         done
                       subgoal
                         apply (rule path_weight_direct_0path[OF dataflow_topology.axioms(1)[OF]])
